proofs/lean/SpecRest/IR.lean
@@ -1,5 +1,13 @@
 namespace SpecRest
 
+inductive TypeExpr where
+  | boolT
+  | intT
+  | enumT (name : String)
+  | entityT (name : String)
+  | relationT (key value : TypeExpr)
+  deriving DecidableEq, Repr, Inhabited
+
 inductive BoolBinOp where
   | and
   | or
@@ -7,7 +15,7 @@ inductive BoolBinOp where
   | iff
   deriving DecidableEq, Repr, Inhabited
 
-inductive IntCmpOp where
+inductive CmpOp where
   | eq
   | neq
   | lt
@@ -23,9 +31,21 @@ inductive Expr where
   | unNot (e : Expr)
   | unNeg (e : Expr)
   | boolBin (op : BoolBinOp) (l r : Expr)
-  | intCmp (op : IntCmpOp) (l r : Expr)
+  | cmp (op : CmpOp) (l r : Expr)
   | letIn (var : String) (value body : Expr)
   | enumAccess (enumName memberName : String)
+  | member (elem : Expr) (relName : String)
+  | forallEnum (var : String) (enumName : String) (body : Expr)
+  deriving Repr, Inhabited
+
+structure FieldDecl where
+  name : String
+  ty : TypeExpr
+  deriving Repr, Inhabited
+
+structure EntityDecl where
+  name : String
+  fields : List FieldDecl
   deriving Repr, Inhabited
 
 structure EnumDecl where
@@ -33,28 +53,37 @@ structure EnumDecl where
   members : List String
   deriving Repr, Inhabited
 
+structure StateScalar where
+  name : String
+  ty : TypeExpr
+  deriving Repr, Inhabited
+
+structure StateRelation where
+  name : String
+  key : TypeExpr
+  value : TypeExpr
+  deriving Repr, Inhabited
+
+structure StateDecl where
+  scalars : List StateScalar
+  relations : List StateRelation
+  deriving Repr, Inhabited
+
 structure InvariantDecl where
   name : String
   body : Expr
   deriving Repr, Inhabited
 
-structure StateField where
-  name : String
-  isInt : Bool
-  deriving Repr, Inhabited
-
-structure StateDecl where
-  fields : List StateField
-  deriving Repr, Inhabited
-
 structure OperationDecl where
   name : String
   requires : List Expr
+  ensures : List Expr
   deriving Repr, Inhabited
 
 structure ServiceIR where
   name : String
   enums : List EnumDecl
+  entities : List EntityDecl
   state : StateDecl
   invariants : List InvariantDecl
   operations : List OperationDecl
